vale/specs/hardware/X64.Print_Inline_s.fst
@@ -1,6 +1,7 @@
 module X64.Print_Inline_s
 
 open X64.Machine_s
+open X64.Bytes_Code_s
 open X64.Bytes_Semantics_s
 open X64.Taint_Semantics_s
 open FStar.IO
